backend/I64Helpers.v
@@ -1,0 +1,165 @@
+
+Require Import Coqlib.
+Require Import AST.
+Require Import Errors.
+Require Import Integers.
+Require Import Floats.
+Require Import Values.
+Require Import Memory.
+Require Import Globalenvs.
+Require Import Events.
+Require Import Cminor.
+Require Import Op.
+
+Require Import mem_lemmas.
+Require Import StructuredInjections.
+Require Import reach.
+
+  (** * Axiomatization of the helper functions *)
+
+Section HELPERS.
+
+Context {F V: Type} (ge: Genv.t (AST.fundef F) V).
+
+Record helper_functions : Type := mk_helper_functions {
+  i64_dtos: ident;                      (**r float -> signed long *)
+  i64_dtou: ident;                      (**r float -> unsigned long *)
+  i64_stod: ident;                      (**r signed long -> float *)
+  i64_utod: ident;                      (**r unsigned long -> float *)
+  i64_stof: ident;                      (**r signed long -> float32 *)
+  i64_utof: ident;                      (**r unsigned long -> float32 *)
+  i64_neg: ident;                       (**r opposite *)
+  i64_add: ident;                       (**r addition *)
+  i64_sub: ident;                       (**r subtraction *)
+  i64_mul: ident;                       (**r multiplication 32x32->64 *)
+  i64_sdiv: ident;                      (**r signed division *)
+  i64_udiv: ident;                      (**r unsigned division *)
+  i64_smod: ident;                      (**r signed remainder *)
+  i64_umod: ident;                      (**r unsigned remainder *)
+  i64_shl: ident;                       (**r shift left *)
+  i64_shr: ident;                       (**r shift right unsigned *)
+  i64_sar: ident                        (**r shift right signed *)
+}.
+
+Variable hf: helper_functions.
+
+Definition hf_names := hf.(i64_dtos)::hf.(i64_dtou) :: 
+  hf.(i64_stod) ::  hf.(i64_utod) :: hf.(i64_stof) ::
+  hf.(i64_utof) :: hf.(i64_neg) :: hf.(i64_add) :: 
+  hf.(i64_sub) :: hf.(i64_mul) :: hf.(i64_sdiv) ::
+  hf.(i64_udiv) :: hf.(i64_smod) :: hf.(i64_umod) ::
+  hf.(i64_shl) :: hf.(i64_shr) :: hf.(i64_sar) :: nil.
+
+
+End HELPERS.
+
+
+Definition sig_l_l := mksignature (Tlong :: nil) (Some Tlong).
+Definition sig_l_f := mksignature (Tlong :: nil) (Some Tfloat).
+Definition sig_l_s := mksignature (Tlong :: nil) (Some Tsingle).
+Definition sig_f_l := mksignature (Tfloat :: nil) (Some Tlong).
+Definition sig_ll_l := mksignature (Tlong :: Tlong :: nil) (Some Tlong).
+Definition sig_li_l := mksignature (Tlong :: Tint :: nil) (Some Tlong).
+Definition sig_ii_l := mksignature (Tint :: Tint :: nil) (Some Tlong).
+
+
+(** Setting up the helper functions *)
+
+Require Import Errors.
+
+Local Open Scope string_scope.
+Local Open Scope error_monad_scope.
+
+Parameter get_helper: String.string -> signature -> res ident.
+Parameter get_builtin: String.string -> signature -> res ident.
+
+Definition get_helpers : res helper_functions :=
+  do i64_dtos <- get_helper "__i64_dtos" sig_f_l ;
+  do i64_dtou <- get_helper "__i64_dtou" sig_f_l ;
+  do i64_stod <- get_helper "__i64_stod" sig_l_f ;
+  do i64_utod <- get_helper "__i64_utod" sig_l_f ;
+  do i64_stof <- get_helper "__i64_stof" sig_l_s ;
+  do i64_utof <- get_helper "__i64_utof" sig_l_s ;
+  do i64_neg <- get_builtin "__builtin_negl" sig_l_l ;
+  do i64_add <- get_builtin "__builtin_addl" sig_ll_l ;
+  do i64_sub <- get_builtin "__builtin_subl" sig_ll_l ;
+  do i64_mul <- get_builtin "__builtin_mull" sig_ll_l ;
+  do i64_sdiv <- get_helper "__i64_sdiv" sig_ll_l ;
+  do i64_udiv <- get_helper "__i64_udiv" sig_ll_l ;
+  do i64_smod <- get_helper "__i64_smod" sig_ll_l ;
+  do i64_umod <- get_helper "__i64_umod" sig_ll_l ;
+  do i64_shl <- get_helper "__i64_shl" sig_li_l ;
+  do i64_shr <- get_helper "__i64_shr" sig_li_l ;
+  do i64_sar <- get_helper "__i64_sar" sig_li_l ;
+  OK (mk_helper_functions
+     i64_dtos i64_dtou i64_stod i64_utod i64_stof i64_utof
+     i64_neg i64_add i64_sub i64_mul i64_sdiv i64_udiv i64_smod i64_umod
+     i64_shl i64_shr i64_sar).
+
+Definition is_I64_helper hf (x:ident) (sg:signature) : bool:=
+  (ident_eq x hf.(i64_dtos) && signature_eq sg sig_f_l) ||
+  (ident_eq x hf.(i64_dtou) && signature_eq sg sig_f_l) ||
+  (ident_eq x hf.(i64_stod) && signature_eq sg sig_l_f) ||
+  (ident_eq x hf.(i64_utod) && signature_eq sg sig_l_f) ||
+  (ident_eq x hf.(i64_stof) && signature_eq sg sig_l_s) ||
+  (ident_eq x hf.(i64_utof) && signature_eq sg  sig_l_s) ||
+  (ident_eq x hf.(i64_neg) && signature_eq sg sig_l_l) ||
+  (ident_eq x hf.(i64_add) && signature_eq sg sig_ll_l) ||
+  (ident_eq x hf.(i64_sub) && signature_eq sg sig_ll_l) ||
+  (ident_eq x hf.(i64_mul) && signature_eq sg sig_ll_l) ||
+  (ident_eq x hf.(i64_sdiv) && signature_eq sg sig_ll_l) ||
+  (ident_eq x hf.(i64_udiv) && signature_eq sg sig_ll_l) ||
+  (ident_eq x hf.(i64_smod) && signature_eq sg sig_ll_l) ||
+  (ident_eq x hf.(i64_umod) && signature_eq sg sig_ll_l) ||
+  (ident_eq x hf.(i64_shl) && signature_eq sg sig_li_l) ||
+  (ident_eq x hf.(i64_shr) && signature_eq sg sig_li_l) ||
+  (ident_eq x hf.(i64_sar) && signature_eq sg sig_li_l).
+
+Inductive is_I64_helperP hf : ident -> signature -> Prop :=
+  ef_dtos: is_I64_helperP hf hf.(i64_dtos) sig_f_l
+| ef_dtou: is_I64_helperP hf hf.(i64_dtou) sig_f_l
+| ef_stod: is_I64_helperP hf hf.(i64_stod) sig_l_f
+| ef_utod: is_I64_helperP hf hf.(i64_utod) sig_l_f
+| ef_stof: is_I64_helperP hf hf.(i64_stof) sig_l_s
+| ef_utof: is_I64_helperP hf hf.(i64_utof)  sig_l_s
+| ef_neg: is_I64_helperP hf hf.(i64_neg) sig_l_l
+| ef_add: is_I64_helperP hf hf.(i64_add) sig_ll_l
+| ef_sub: is_I64_helperP hf hf.(i64_sub) sig_ll_l
+| ef_mul: is_I64_helperP hf hf.(i64_mul) sig_ll_l
+| ef_sdiv: is_I64_helperP hf hf.(i64_sdiv) sig_ll_l
+| ef_udiv: is_I64_helperP hf hf.(i64_udiv) sig_ll_l
+| ef_smod: is_I64_helperP hf hf.(i64_smod) sig_ll_l
+| ef_umod: is_I64_helperP hf hf.(i64_umod) sig_ll_l
+| ef_shl: is_I64_helperP hf hf.(i64_shl) sig_li_l
+| ef_shr: is_I64_helperP hf hf.(i64_shr) sig_li_l
+| ef_sarf: is_I64_helperP hf hf.(i64_sar) sig_li_l.
+
+Lemma identeq_and x b: ((ident_eq x x) && b) = b.
+Proof. destruct (ident_eq x x); intuition. Qed. 
+Lemma sigeq_or x b: ((signature_eq x x) || b) = true.
+Proof. destruct (signature_eq x x); intuition. Qed. 
+Lemma sigeq_or' x b: (b || (signature_eq x x)) = true.
+Proof. destruct (signature_eq x x); intuition. Qed. 
+
+Lemma ident_sig_eq_elim b name name' sg sg': 
+  ((b || (ident_eq name name' && signature_eq sg sg')) = true)
+<->
+  (b=true \/ (name=name' /\ sg=sg')).
+Proof.
+destruct b; simpl. intuition. 
+destruct (ident_eq name name'); simpl.
+destruct (signature_eq sg sg'); simpl. intuition. intuition. intuition. 
+Qed.
+
+Lemma is64helper_char hf (name:ident) (sg:signature) :
+   is_I64_helperP hf name sg <-> (is_I64_helper hf name sg = true).
+Proof.
+split; intros.
+unfold is_I64_helper.
+inv H; rewrite identeq_and; try rewrite sigeq_or'; trivial. 
+unfold is_I64_helper in H. 
+  repeat rewrite ident_sig_eq_elim in H.
+  intuition; try solve [subst; constructor]. 
+    destruct (ident_eq name (i64_dtos hf)); try inv H.
+    destruct (signature_eq sg sig_f_l); try inv H1. constructor.
+Qed.
