backend/LTL_eff.v
@@ -110,7 +110,8 @@ Inductive ltl_effstep (g:genv):  (block -> Z -> bool) ->
         (LTL_State s f (Vptr sp Int.zero) f.(fn_entrypoint) rs') m'
 
   | ltl_effstep_function_external: forall s ef t args res rs m rs' m'
-      (OBS: observableEF hf ef = false),
+      (*(OBS: observableEF hf ef = false),*)
+      (OBS: EFisHelper hf ef = true),
       args = map rs (loc_arguments (ef_sig ef)) ->
       external_call' ef g args m t res m' ->
       rs' = Locmap.setlist (map R (loc_result (ef_sig ef))) res rs ->
@@ -162,13 +163,19 @@ intros.
   split. unfold corestep, coopsem; simpl. econstructor; eassumption.
          eapply FreeEffect_free; eassumption. 
   split. unfold corestep, coopsem; simpl. econstructor; eassumption.
-         eapply Mem.alloc_unchanged_on; eassumption. 
-  split. unfold corestep, coopsem; simpl. econstructor; eassumption.
+         eapply Mem.alloc_unchanged_on; eassumption.
+  split. unfold corestep, coopsem; simpl. 
+         eapply ltl_exec_function_external; eassumption.
          inv H0.
-         eapply mem_unchanged_on_sub.
-           eapply BuiltinEffect_unchOn; eassumption. 
-         simpl. unfold BuiltinEffect. intros.
-           destruct ef; trivial. 
+         destruct ef; try inv OBS.
+           eapply mem_unchanged_on_sub.
+             eapply BuiltinEffect_unchOn; try eapply H2. 
+              instantiate(1:=hf). unfold observableEF. rewrite H0. trivial.
+             unfold BuiltinEffect; simpl; intros. trivial.
+           eapply mem_unchanged_on_sub.
+             eapply BuiltinEffect_unchOn; try eapply H2. 
+              instantiate(1:=hf). unfold observableEF. rewrite H0. trivial.
+             unfold BuiltinEffect; simpl; intros. trivial.
   split. unfold corestep, coopsem; simpl. econstructor; eassumption.
          apply Mem.unchanged_on_refl.
 Qed.
