backend/Mach_coop.v
@@ -409,7 +409,7 @@ Lemma store_args_rec_succeeds_aux sz m sp args tys z
   Mem.range_perm m sp (4*z) (4*z + 4*sz) Cur Writable -> 
   exists m', store_args_rec m sp z args tys = Some m'.
 Proof.
-Admitted. (*TODO*)
+Admitted. (*TODO Gordon*)
 
 Lemma store_args_rec_succeeds sz m sp args tys 
       (VALSDEF: val_casted.vals_defined args=true)
@@ -627,7 +627,8 @@ Inductive mach_step (ge:genv): Mach_core -> mem -> Mach_core -> mem -> Prop :=
 *)
   | Mach_exec_function_external:
       forall cs f' rs m t rs' callee args res m' lf
-      (OBS: observableEF hf callee = false),
+(*     (OBS: observableEF hf callee = false),*)
+      (OBS: EFisHelper hf callee = true),
       Genv.find_funct_ptr ge f' = Some (External callee) ->
       external_call' callee ge args m t res m' ->
       rs' = set_regs (loc_result (ef_sig callee)) res rs ->
@@ -744,7 +745,10 @@ Lemma Mach_after_at_external_excl : forall retv q q',
 Lemma Mach_corestep_not_at_external ge m q m' q':
       mach_step ge q m q' m' -> Mach_at_external q = None.
 Proof. intros. inv H; try reflexivity. 
-  simpl. rewrite OBS. trivial. Qed.
+  simpl. unfold observableEF. unfold EFisHelper in OBS.  
+  destruct callee; try inv OBS. 
+  rewrite H2. trivial. rewrite H2. trivial.  
+Qed.  
 
 Lemma Mach_corestep_not_halted ge m q m' q': 
       mach_step ge q m q' m' -> Mach_halted q = None.
